{
 "cells": [
  {
   "cell_type": "markdown",
   "id": "e6296f2f",
   "metadata": {},
   "source": [
    "## Exercise 2: Linear Systems In Three Unknowns"
   ]
  },
  {
   "cell_type": "markdown",
   "id": "747f292e",
   "metadata": {},
   "source": [
    "> 1. Find the unique solution to the system of equations.\n",
    "\n",
    "\\begin{gather*}\n",
    "    2x + y - z = 3 \\\\\n",
    "    x - y + z = 0 \\\\\n",
    "    x - 2y - 3z = 4 \\\\ \\\\\n",
    "\n",
    "    x - y + z = 0 \\\\\n",
    "    x = y - z \\\\ \\\\\n",
    "\n",
    "    2x + y - z = 3 \\\\\n",
    "    2(y - z) + y - z = 3 \\\\\n",
    "    2y - 2z + y - z = 3 \\\\\n",
    "    3y - 3z = 3 \\\\\n",
    "    y - z = 1 \\\\ \\\\\n",
    "\n",
    "    x - 2y - 3z = 4 \\\\\n",
    "    (y - z) - 2y - 3z = 4 \\\\\n",
    "    y - z - 2y - 3z = 4 \\\\\n",
    "    -y - 4z = 4 \\\\ \\\\\n",
    "\n",
    "    y - z = 1 \\\\\n",
    "    + (-y - 4z = 4) \\\\\n",
    "    -5z = 5 \\\\\n",
    "    \\frac{-5z = 5}{-5} \\\\\n",
    "    \\boxed{z = -1} \\\\ \\\\\n",
    "\n",
    "    x = y - z \\\\\n",
    "    x = y - (-1) \\\\\n",
    "    x = y + 1 \\\\ \\\\\n",
    "\n",
    "    2(y + 1) + y - (-1) = 3 \\\\\n",
    "    2y + 2 + y + 1 = 3 \\\\\n",
    "    3y + 3 = 3 \\\\\n",
    "    3y = 3 - 3 \\\\\n",
    "    \\boxed{y = 0} \\\\ \\\\\n",
    "\n",
    "    x - 2y - 3z = 4 \\\\\n",
    "    x - 2(0) - 3(-1) = 4 \\\\\n",
    "    x - 0 + 3 = 4 \\\\\n",
    "    x + 3 = 4 \\\\\n",
    "    x = 4 - 3 \\\\\n",
    "    \\boxed{x = 1} \\\\ \\\\\n",
    "\n",
    "    \\boxed{(x, y, z) = (1, 0, -1)} \\\\ \\\\\n",
    "\n",
    "    \\textbf{CHECKING} \\\\\n",
    "    2x + y - z = 3 \\\\\n",
    "    2(1) + (0) - (-1) = 3 \\\\\n",
    "    2 + 0 + 1 = 3 \\\\\n",
    "    2 + 1 = 3 \\\\\n",
    "    3 = 3 \\\\ \\\\\n",
    "\n",
    "    x - y + z = 0 \\\\\n",
    "    (1) - (0) + (-1) = 0 \\\\\n",
    "    1 - 0 - 1 = 0 \\\\\n",
    "    1 - 1 = 0 \\\\\n",
    "    0 = 0 \\\\ \\\\\n",
    "\n",
    "    x - 2y - 3z = 4 \\\\\n",
    "    (1) - 2(0) - 3(-1) = 4 \\\\\n",
    "    1 - 0 + 3 = 4 \\\\\n",
    "    1 + 3 = 4 \\\\\n",
    "    4 = 4\n",
    "\\end{gather*}"
   ]
  },
  {
   "cell_type": "markdown",
   "id": "bbba5fa9",
   "metadata": {},
   "source": [
    "> 2. Find the unique solution to the system of equations.\n",
    "\n",
    "\\begin{gather*}\n",
    "    3x + y - z = -2 \\\\\n",
    "    x - 2y + 3z = 23 \\\\\n",
    "    2x + 3y + 2z = 5 \\\\ \\\\\n",
    "\n",
    "    x - 2y + 3z = 23 \\\\\n",
    "    3x + y - z = -2 \\\\\n",
    "    2x + 3y + 2z = 5 \\\\ \\\\\n",
    "\n",
    "    3(x - 2y + 3z = 23) \\\\\n",
    "    + -(3x + y - z = -2) \\\\ \\\\\n",
    "\n",
    "    3x - 6y + 9z = 69 \\\\\n",
    "    + (-3x - y + z = 2) \\\\\n",
    "    -7y + 10z = 71 \\\\ \\\\\n",
    "\n",
    "    2(x - 2y + 3z = 23) \\\\\n",
    "    + -(2x + 3y + 2z = 5) \\\\ \\\\\n",
    "\n",
    "    2x - 4y + 6z = 46 \\\\\n",
    "    + (-2x - 3y - 2z = -5) \\\\\n",
    "    -7y + 4z = 41 \\\\ \\\\\n",
    "\n",
    "    -7y + 10z = 71 \\\\\n",
    "    + -(-7y + 4z = 41) \\\\ \\\\\n",
    "    \n",
    "    -7y + 10z = 71 \\\\\n",
    "    + (7y - 4z = -41) \\\\\n",
    "    6z = 30 \\\\\n",
    "    \\frac{6z = 30}{6} \\\\\n",
    "    \\boxed{z = 5} \\\\ \\\\\n",
    "\n",
    "    x - 2y + 3(5) = 23 \\\\\n",
    "    x - 2y + 15 = 23 \\\\\n",
    "    x - 2y = 23 - 15 \\\\\n",
    "    x - 2y = 8 \\\\ \\\\\n",
    "\n",
    "    3x + y - z = -2 \\\\\n",
    "    3x + y - (5) = -2 \\\\\n",
    "    3x + y - 5 = -2 \\\\\n",
    "    3x + y = 5 - 2 \\\\\n",
    "    3x + y = 3 \\\\ \\\\\n",
    "\n",
    "    2x + 3y + 2z = 5 \\\\\n",
    "    2x + 3y + 2(5) = 5 \\\\\n",
    "    2x + 3y + 10 = 5 \\\\\n",
    "    2x + 3y = 5 - 10 \\\\ \n",
    "    2x + 3y = -5 \\\\ \\\\\n",
    "\n",
    "    x - 2y = 8 \\\\\n",
    "    x = 2y + 8 \\\\ \\\\\n",
    "\n",
    "    3x + y = 3 \\\\\n",
    "    3(2y + 8) + y = 3 \\\\\n",
    "    6y + 24 + y = 3 \\\\\n",
    "    7y + 24 = 3 \\\\\n",
    "    7y = 3 - 24 \\\\\n",
    "    7y = -21 \\\\\n",
    "    \\frac{7y = -21}{7} \\\\\n",
    "    \\boxed{y = -3} \\\\ \\\\\n",
    "\n",
    "    2x + 3y = -5 \\\\\n",
    "    2x + 3(-3) = -5 \\\\\n",
    "    2x - 9 = -5 \\\\\n",
    "    2x = 9 - 5 \\\\\n",
    "    2x = 4 \\\\\n",
    "    \\frac{2x = 4}{2} \\\\\n",
    "    \\boxed{x = 2} \\\\ \\\\\n",
    "\n",
    "    \\boxed{(x, y, z) = (2, -3, 5)} \\\\ \\\\\n",
    "\n",
    "    \\textbf{CHECKING} \\\\\n",
    "    3x + y - z = -2 \\\\\n",
    "    3(2) + (-3) - (5) = -2 \\\\\n",
    "    6 - 3 - 5 = -2 \\\\\n",
    "    3 - 5 = -2 \\\\\n",
    "    -2 = -2 \\\\ \\\\\n",
    "    \n",
    "    x - 2y + 3z = 23 \\\\\n",
    "    (2) - 2(-3) + 3(5) = 23 \\\\\n",
    "    2 + 6 + 15 = 23 \\\\\n",
    "    8 + 15 = 23 \\\\\n",
    "    23 = 23 \\\\ \\\\\n",
    "\n",
    "    2x + 3y + 2z = 5 \\\\ \n",
    "    2(2) + 3(-3) + 2(5) = 5 \\\\\n",
    "    4 - 9 + 10 = 5 \\\\\n",
    "    -5 + 10 = 5 \\\\\n",
    "    5 = 5\n",
    "\\end{gather*}"
   ]
  },
  {
   "cell_type": "markdown",
   "id": "072ba8c0",
   "metadata": {},
   "source": [
    "> 3. Find the unique solution to the system of equations.\n",
    "\n",
    "\\begin{gather*}\n",
    "    5x - 3y + z = -8 \\\\\n",
    "    2x + y - 2z = -6 \\\\\n",
    "    -3x + 2y + 4z = 19 \\\\ \\\\\n",
    "\n",
    "    2x + y - 2z = -6 \\\\\n",
    "    5x - 3y + z = -8 \\\\\n",
    "    -3x + 2y + 4z = 19 \\\\ \\\\\n",
    "\n",
    "    2x + y - 2z = -6 \\\\\n",
    "    \\frac{2x + y - 2z = -6}{2} \\\\\n",
    "    x + \\frac{1}{2}y - z = -3 \\\\ \\\\\n",
    "\n",
    "    5(x + \\frac{1}{2}y - z = -3) \\\\\n",
    "    + -(5x - 3y + z = -8) \\\\ \\\\\n",
    "\n",
    "    5x + \\frac{5}{2}y - 5z = -15 \\\\\n",
    "    + (-5x + \\frac{6}{2}y - z = 8) \\\\\n",
    "    \\frac{11}{2}y - 6z = -7 \\\\ \\\\\n",
    "\n",
    "    3(x + \\frac{1}{2}y - z = -3) \\\\\n",
    "    + (-3x + 2y + 4z = 19) \\\\ \\\\\n",
    "\n",
    "    3x + \\frac{3}{2}y - 3z = -9\n",
    "    + (-3x + \\frac{4}{2}y + 4z = 19) \\\\\n",
    "    \\frac{7}{2}y + z = 10 \\\\ \\\\\n",
    "\n",
    "    \\frac{11}{2}y - 6z = -7 \\\\\n",
    "    + 6(\\frac{7}{2}y + z = 10) \\\\ \\\\\n",
    "\n",
    "    \\frac{11}{2}y - 6z = -7 \\\\\n",
    "    + (\\frac{42}{2}y + 6z = 60) \\\\\n",
    "    \\frac{53}{2}y = 53 \\\\\n",
    "    \\frac{2}{53}(\\frac{53}{2}y = 53) \\\\\n",
    "    y = \\frac{106}{53} \\\\\n",
    "    \\boxed{y = 2} \\\\ \\\\\n",
    "\n",
    "    x + \\frac{1}{2}y - z = -3 \\\\\n",
    "    x + \\frac{2}{2}y - z = -3 \\\\\n",
    "    x + 1 - z = -3 \\\\\n",
    "    x - z = -3 - 1 \\\\\n",
    "    x - z = -4 \\\\\n",
    "    x = z - 4 \\\\ \\\\\n",
    "\n",
    "    5x - 3y + z = -8 \\\\\n",
    "    5(z - 4) - 3(2) + z = -8 \\\\\n",
    "    5z - 20 - 6 + z = -8 \\\\\n",
    "    6z - 26 = -8 \\\\\n",
    "    6z = 26 - 8 \\\\\n",
    "    6z = 18 \\\\\n",
    "    \\frac{6z = 18}{6} \\\\\n",
    "    \\boxed{z = 3} \\\\ \\\\\n",
    "\n",
    "    -3x + 2y + 4z = 19 \\\\\n",
    "    -3x + 2(2) + 4(3) = 19 \\\\\n",
    "    -3x + 4 + 12 = 19 \\\\\n",
    "    -3x + 16 = 19 \\\\\n",
    "    -3x = 19 - 16 \\\\\n",
    "    -3x = 3 \\\\\n",
    "    \\frac{-3x = 3}{-3} \\\\\n",
    "    \\boxed{x = -1} \\\\ \\\\\n",
    "\n",
    "    \\boxed{(x, y, z) = (-1, 2, 3)} \\\\ \\\\\n",
    "\n",
    "    \\textbf{CHECKING} \\\\\n",
    "    5x - 3y + z = -8 \\\\\n",
    "    5(-1) - 3(2) + (3) = -8 \\\\\n",
    "    -5 - 6 + 3 = -8 \\\\\n",
    "    -11 + 3 = -8 \\\\\n",
    "    -8 = -8 \\\\ \\\\\n",
    "\n",
    "    2x + y - 2z = -6 \\\\\n",
    "    2(-1) + (2) - 2(3) = -6 \\\\\n",
    "    -2 + 2 - 6 = -6 \\\\\n",
    "    0 - 6 = -6 \\\\\n",
    "    -6 = -6 \\\\ \\\\\n",
    "\n",
    "    -3x + 2y + 4z = 19 \\\\ \n",
    "    -3(-1) + 2(2) + 4(3) = 19 \\\\\n",
    "    3 + 4 + 12 = 19 \\\\\n",
    "    7 + 12 = 19 \\\\\n",
    "    19 = 19\n",
    "\\end{gather*}"
   ]
  },
  {
   "cell_type": "markdown",
   "id": "2f1f62fa",
   "metadata": {},
   "source": [
    "> 4. Find the unique solution to the system of equations.\n",
    "\n",
    "\\begin{gather*}\n",
    "    -2x + 3y - 4z = 10 \\\\\n",
    "    4x + 3y + 2z = 4 \\\\\n",
    "    x - 6y + 4z = -19 \\\\ \n",
    "\\end{gather*}"
   ]
  },
  {
   "cell_type": "markdown",
   "id": "03214b92",
   "metadata": {},
   "source": [
    "> 5. Find the unique solution to the system of equations.\n",
    "\n",
    "\\begin{gather*}\n",
    "    2x - y + z = 9 \\\\\n",
    "    4x - 2y + 2z = 18 \\\\\n",
    "    -2x + y - z = -9 \\\\ \n",
    "\\end{gather*}"
   ]
  },
  {
   "cell_type": "markdown",
   "id": "822168d1",
   "metadata": {},
   "source": [
    "> 6. Find the unique solution to the system of equations.\n",
    "\n",
    "\\begin{gather*}\n",
    "    x + 2y - z = 9 \\\\\n",
    "    3x + y - z = 5 \\\\\n",
    "    -x - 4y + z = 2 \\\\ \n",
    "\\end{gather*}"
   ]
  }
 ],
 "metadata": {
  "language_info": {
   "name": "python"
  }
 },
 "nbformat": 4,
 "nbformat_minor": 5
}
