{
 "cells": [
  {
   "cell_type": "markdown",
   "id": "ca17bf7f",
   "metadata": {},
   "source": [
    "## Quiz 2: Linear Systems In Three Unknowns"
   ]
  },
  {
   "cell_type": "markdown",
   "id": "4cfa2c00",
   "metadata": {},
   "source": [
    "> 1. Use any method to find the solution to the system of equations.\n",
    "\n",
    "\\begin{gather*}\n",
    "    x + y - z = 4 \\\\\n",
    "    x - y - z = 2 \\\\\n",
    "    x + 2y + z = 1 \\\\ \\\\\n",
    "\n",
    "    x + y - z = 4 \\\\\n",
    "    + (x - y - z = 2) \\\\ \\\\\n",
    "\n",
    "    2x - 2z = 6 \\sim \\boxed{x - z = 3 \\ \\text{or} \\ x = z + 3} \\\\ \\\\\n",
    "\n",
    "    x + 2y + z = 1 \\\\\n",
    "    + -2(x + y - z = 4) \\\\ \\\\\n",
    "\n",
    "    x + 2y + z = 1 \\\\\n",
    "    + (-2x - 2y + 2z = -8) \\\\ \\\\\n",
    "\n",
    "    -x + 3z = -7 \\sim \\boxed{x = 3z + 7} \\\\ \\\\\n",
    "\n",
    "    z + 3 = 3z + 7 \\\\\n",
    "    -7 + 3 = 3z - z \\\\\n",
    "    -4 = 2z \\\\\n",
    "    \\boxed{z = -2} \\\\ \\\\\n",
    "\n",
    "    x = z + 3 \\\\\n",
    "    x = (-2) + 3 \\\\\n",
    "    \\boxed{x = 1} \\\\ \\\\\n",
    "\n",
    "    x + y - z = 4 \\\\\n",
    "    (1) + y - (-2) = 4 \\\\\n",
    "    y + 3 = 4 \\\\\n",
    "    y = 4 - 3 \\\\\n",
    "    \\boxed{y = 1} \\\\ \\\\\n",
    "\n",
    "    \\textbf{CHECKING} \\\\\n",
    "    x + y - z = 4 \\\\\n",
    "    (1) + (1) - (-2) = 4 \\\\\n",
    "    2 + 2 = 4 \\\\\n",
    "    \\boxed{4 = 4} \\\\ \\\\\n",
    "\n",
    "    x - y - z = 2 \\\\\n",
    "    (1) - (1) - (-2) = 2 \\\\\n",
    "    \\boxed{2 = 2} \\\\ \\\\\n",
    "\n",
    "    x + 2y + z = 1 \\\\\n",
    "    (1) + 2(1) + (-2) = 1 \\\\\n",
    "    1 + 2 - 2 = 1 \\\\\n",
    "    \\boxed{1 = 1} \\\\ \\\\\n",
    "\n",
    "    \\boxed{(x, y, z) = (1, 1, -2)}\n",
    "\\end{gather*}"
   ]
  },
  {
   "cell_type": "markdown",
   "id": "9519f39b",
   "metadata": {},
   "source": [
    "> 2. Use any method to find the solution to the linear system.\n",
    "\n",
    "\\begin{gather*}\n",
    "    x - y + z = -6 \\\\\n",
    "    3x - 4y - z = -4 \\\\\n",
    "    -2x + 3y + 4z = 14 \\\\ \\\\\n",
    "\n",
    "    3(x - y + z = -6) \\\\\n",
    "    - (3x - 4y - z = -4) \\\\ \\\\\n",
    "\n",
    "    3x - 3y + 3z = -18 \\\\\n",
    "    - (3x - 4y - z = -4) \\\\ \\\\\n",
    "    \n",
    "    y + 4z = -14 \\sim \\boxed{y = -4z - 14} \\\\ \\\\\n",
    "    \n",
    "    -2x + 3y + 4z = 14 \\\\\n",
    "    - -2(x - y + z = -6) \\\\ \\\\\n",
    "    \n",
    "    -2x + 3y + 4z = 14 \\\\\n",
    "    - -2x + 2y - 2z = 12 \\\\ \\\\\n",
    "\n",
    "    y + 6z = 2 \\sim \\boxed{y = -6z + 2} \\\\ \\\\\n",
    "\n",
    "    -4z - 14 = -6z + 2 \\\\\n",
    "    6z - 4z = 14 + 2 \\\\\n",
    "    2z = 16 \\\\\n",
    "    \\boxed{z = 8} \\\\ \\\\\n",
    "\n",
    "    y = -4z - 14 \\\\\n",
    "    y = -4(8) - 14 \\\\\n",
    "    y = -32 - 14 \\\\\n",
    "    \\boxed{y = -46} \\\\ \\\\\n",
    "\n",
    "    x - y + z = -6 \\\\\n",
    "    x - (-46) + (8) = -6 \\\\\n",
    "    x + 46 + 8 = -6\n",
    "    x + 54 = -6 \\\\\n",
    "    x = -54 - 6 \\\\\n",
    "    \\boxed{x = -60} \\\\ \\\\\n",
    "\n",
    "    \\textbf{CHECKING} \\\\\n",
    "    x - y + z = -6 \\\\\n",
    "    (-60) - (-46) + (8) = -6 \\\\\n",
    "    -60 + 46 + 8 = -6 \\\\\n",
    "    -14 + 8 = -6 \\\\\n",
    "    \\boxed{-6 = -6} \\\\ \\\\\n",
    "\n",
    "    3x - 4y - z = -4 \\\\\n",
    "    3(-60) - 4(-46) - (8) = -4 \\\\\n",
    "    -180 + 184 - 8 = -4 \\\\\n",
    "    4 - 8 = -4 \\\\\n",
    "    \\boxed{-4 = -4} \\\\ \\\\\n",
    "\n",
    "    -2x + 3y + 4z = 14 \\\\\n",
    "    -2(-60) + 3(-46) + 4(8) = 14 \\\\\n",
    "    120 - 138 + 32 = 14 \\\\\n",
    "    -18 + 32 = 14 \\\\\n",
    "    \\boxed{14 = 14} \\\\ \\\\\n",
    "\n",
    "    \\boxed{(x, y, z) = (-60, -46, 8)}\n",
    "\\end{gather*}"
   ]
  },
  {
   "cell_type": "markdown",
   "id": "699643fa",
   "metadata": {},
   "source": [
    "> 3. Solve the system for $x$, $y$, and $z$.\n",
    "\n",
    "\\begin{gather*}\n",
    "    x + 2z = 3 \\\\\n",
    "    3x - 2y + z = -11 \\\\\n",
    "    2x + y + 3z = 9 \\\\ \\\\\n",
    "    \n",
    "    3x - 2y + z = -11 \\\\\n",
    "    + 2(2x + y + 3z = 9) \\\\ \\\\\n",
    "\n",
    "    3x - 2y + z = -11 \\\\\n",
    "    + (4x + 2y + 6z = 18) \\\\ \\\\\n",
    "\n",
    "    7x + 7z = 7 \\sim \\boxed{x = -z + 1} \\\\ \\\\\n",
    "\n",
    "    x + 2z = 3 \\sim x = -2z + 3 \\\\\n",
    "    -z + 1 = -2z + 3 \\\\\n",
    "    2z - z = 3 - 1 \\\\\n",
    "    \\boxed{z = 2} \\\\ \\\\\n",
    "\n",
    "    x = -(2) + 1 \\\\\n",
    "    x = -2 + 1 \\\\\n",
    "    \\boxed{x = -1} \\\\ \\\\\n",
    "\n",
    "    3x - 2y + z = -11 \\\\\n",
    "    3(-1) - 2y + (2) = -11 \\\\\n",
    "    -3 - 2y + 2 = -11 \\\\\n",
    "    -3 + 2 + 11 = 2y \\\\\n",
    "    10 = 2y \\\\\n",
    "    \\boxed{y = 5} \\\\ \\\\\n",
    "\n",
    "    \\textbf{CHECKING} \\\\\n",
    "    x + 2z = 3 \\\\\n",
    "    (-1) + 2(2) = 3 \\\\\n",
    "    -1 + 4 = 3 \\\\\n",
    "    \\boxed{3 = 3} \\\\ \\\\\n",
    "\n",
    "    3x - 2y + z = -11 \\\\\n",
    "    3(-1) - 2(5) + (2) = -11 \\\\\n",
    "    -3 - 10 + 2 = -11 \\\\\n",
    "    -13 + 2 = -11 \\\\\n",
    "    \\boxed{-11 = -11} \\\\ \\\\\n",
    "\n",
    "    2x + y + 3z = 9 \\\\\n",
    "    2(-1) + (5) + 3(2) = 9 \\\\\n",
    "    -2 + 5 + 6 = 9 \\\\\n",
    "    3 + 6 = 9 \\\\\n",
    "    \\boxed{9 = 9} \\\\ \\\\\n",
    "\n",
    "    \\boxed{(x, y, z) = (-1, 5, 2)}\n",
    "\\end{gather*}"
   ]
  }
 ],
 "metadata": {
  "language_info": {
   "name": "python"
  }
 },
 "nbformat": 4,
 "nbformat_minor": 5
}
